Extend Normalform type class with property nf_impure, #45

Coq/src/Classes.v
@@ -7,5 +7,8 @@ Class Shareable (A : Type) :=
 
 Class Normalform (A B : Type) :=
   {
-    nf : Prog A -> Prog B
+    nf : Prog A -> Prog B;
+    nf_impure: forall s (pf : _ -> Prog A),
+        nf (impure (ext s pf)) = impure (ext s (fun p => nf (pf p)))
+
   }.
